Impl/JournalistModel.i.dfy
@@ -1,13 +1,16 @@
 include "../ByteBlockCacheSystem/JournalBytes.i.dfy"
 include "../BlockCacheSystem/DiskLayout.i.dfy"
+include "JournalistMarshallingModel.i.dfy"
 
 module JournalistModel {
-  import opened JournalRanges
-  import opened JournalBytes
-  import opened Journal
   import opened DiskLayout
   import opened NativeTypes
   import opened Options
+
+  import opened JournalRanges`Internal
+  import opened JournalBytes
+  import opened Journal
+  import opened JournalistMarshallingModel
 
   datatype JournalInfo = JournalInfo(
     inMemoryJournalFrozen: seq<JournalEntry>,
@@ -15,46 +18,53 @@ module JournalistModel {
     replayJournal: seq<JournalEntry>,
 
     journalFrontRead: Option<JournalRange>,
-    journalBackRead: Option<JournalRange>
+    journalBackRead: Option<JournalRange>,
+
+    ghost writtenLen: int
   )
 
   datatype JournalistModel = JournalistModel(
     journalEntries: seq<JournalEntry>,
-    fStart: uint64,
-    fLen: uint64,
-    eStart: uint64,
-    eLen: uint64,
+    start: uint64,
+    len1: uint64,
+    len2: uint64,
 
     replayJournal: seq<JournalEntry>,
     replayIdx: uint64,
 
     journalFrontRead: Option<seq<byte>>,
-    journalBackRead: Option<seq<byte>>)
+    journalBackRead: Option<seq<byte>>,
+    
+    // number of blocks already written on disk:
+    writtenJournalBlocks: uint64,
+    // number of *blocks* of inMemoryJournalFrozen:
+    frozenJournalBlocks: uint64,
+    // number of *bytes* of inMemoryJournal:
+    inMemoryWeight: uint64
+  )
 
   function method Len() : uint64 { 1048576 }
+
+  function method basic_mod(x: uint64) : uint64
+  {
+    if x >= Len() then x - Len() else x
+  }
 
   predicate WF(jm: JournalistModel)
   {
     && |jm.journalEntries| == Len() as int
-    && 0 <= jm.fStart < Len()
-    && 0 <= jm.fLen <= Len()
-    && 0 <= jm.eStart < Len()
-    && 0 <= jm.eLen <= Len()
+    && 0 <= jm.start < Len()
+    && 0 <= jm.len1 <= Len()
+    && 0 <= jm.len2 <= Len()
+    && 0 <= jm.len1 + jm.len2 <= Len()
     && 0 <= jm.replayIdx as int <= |jm.replayJournal|
     && (jm.journalFrontRead.Some? ==>
         JournalRangeOfByteSeq(jm.journalFrontRead.value).Some?)
     && (jm.journalBackRead.Some? ==>
         JournalRangeOfByteSeq(jm.journalBackRead.value).Some?)
-  }
-
-  function cyclicSlice<T>(t: seq<T>, start: uint64, l: uint64) : seq<T>
-  requires 0 <= start as int < |t|
-  requires 0 <= l as int <= |t|
-  {
-    if start as int + l as int <= |t| then
-      t[start .. start + l]
-    else
-      t[start ..] + t[.. start + l - |t| as uint64]
+    && 0 <= jm.writtenJournalBlocks <= NumJournalBlocks()
+    && 0 <= jm.frozenJournalBlocks <= NumJournalBlocks()
+    && 0 <= jm.inMemoryWeight <= NumJournalBlocks() * 4096
   }
 
   function IJournalRead(j: Option<seq<byte>>) : Option<JournalRange>
@@ -62,16 +72,165 @@ module JournalistModel {
   {
     if j.Some? then JournalRangeOfByteSeq(j.value) else None
   }
-    
+
+  function start(jm: JournalistModel) : uint64
+  {
+    jm.start
+  }
+
+  function mid(jm: JournalistModel) : uint64
+  requires jm.start < Len()
+  requires jm.len1 <= Len()
+  {
+    basic_mod(jm.start + jm.len1)
+  }
+
+  function end(jm: JournalistModel) : uint64
+  requires jm.start < Len()
+  requires jm.len1 <= Len()
+  requires jm.len2 <= Len()
+  {
+    basic_mod(jm.start + jm.len1 + jm.len2)
+  }
+
+  function InMemoryJournalFrozen(jm: JournalistModel) : seq<JournalEntry>
+  requires WF(jm)
+  {
+    cyclicSlice(jm.journalEntries, start(jm), jm.len1)
+  }
+
+  function InMemoryJournal(jm: JournalistModel) : seq<JournalEntry>
+  requires WF(jm)
+  {
+    cyclicSlice(jm.journalEntries, mid(jm), jm.len2)
+  }
+
+  function ReplayJournal(jm: JournalistModel) : seq<JournalEntry>
+  requires 0 <= jm.replayIdx as int <= |jm.replayJournal|
+  {
+    jm.replayJournal[jm.replayIdx..]
+  }
+
+  function JournalFrontRead(jm: JournalistModel) : Option<JournalRange>
+  requires WF(jm)
+  {
+    IJournalRead(jm.journalFrontRead)
+  }
+
+  function JournalBackRead(jm: JournalistModel) : Option<JournalRange>
+  requires WF(jm)
+  {
+    IJournalRead(jm.journalBackRead)
+  }
+
+  function WrittenJournalLen(jm: JournalistModel) : int
+  {
+    jm.writtenJournalBlocks as int
+  }
+
   protected function I(jm: JournalistModel) : JournalInfo
   requires WF(jm)
   {
     JournalInfo(
-      cyclicSlice(jm.journalEntries, jm.fStart, jm.fLen),
-      cyclicSlice(jm.journalEntries, jm.eStart, jm.eLen),
-      replayJournal[replayIdx..],
-      IJournalRead(jm.journalFrontRead),
-      IJournalRead(jm.journalBackRead)
+      InMemoryJournalFrozen(jm),
+      InMemoryJournal(jm),
+      ReplayJournal(jm),
+      JournalFrontRead(jm),
+      JournalBackRead(jm),
+      WrittenJournalLen(jm)
     )
+  }
+
+  predicate Inv(jm: JournalistModel)
+  {
+    && WF(jm)
+    && (jm.writtenJournalBlocks + jm.frozenJournalBlocks) * 4064 +
+        jm.inMemoryWeight <= 4064 * NumJournalBlocks()
+    && WeightJournalEntries(InMemoryJournalFrozen(jm)) <= jm.frozenJournalBlocks as int * 4064
+    && WeightJournalEntries(InMemoryJournal(jm)) == jm.inMemoryWeight as int
+  }
+
+  ///// Steps you can take
+
+  function {:opaque} hasFrozenJournal(jm: JournalistModel) : (b: bool)
+  requires Inv(jm)
+  ensures b == (I(jm).inMemoryJournalFrozen == [])
+  {
+    jm.len1 == 0    
+  }
+
+  function {:opaque} packageFrozenJournal(jm: JournalistModel)
+      : (res : (JournalistModel, seq<byte>))
+  requires Inv(jm)
+  requires I(jm).inMemoryJournalFrozen != []
+  ensures var (jm', s) := res;
+    && Inv(jm')
+    && JournalRangeOfByteSeq(s).Some?
+    && parseJournalRange(JournalRangeOfByteSeq(s).value) == Some(I(jm).inMemoryJournalFrozen)
+    && I(jm') == I(jm)
+          .(inMemoryJournalFrozen := [])
+          .(writtenLen := I(jm).writtenLen
+                + |JournalRangeOfByteSeq(s).value|)
+  {
+    var s := marshallJournalEntries(jm.journalEntries, jm.start, jm.len1, jm.frozenJournalBlocks);
+    var jm' := jm.(start := basic_mod(jm.start + jm.len1))
+                 .(len1 := 0)
+                 .(frozenJournalBlocks := 0)
+                 .(writtenJournalBlocks := jm.writtenJournalBlocks + jm.frozenJournalBlocks);
+    (jm', s)
+  }
+
+  function {:opaque} packageInMemoryJournal(jm: JournalistModel)
+      : (res : (JournalistModel, seq<byte>))
+  requires Inv(jm)
+  requires I(jm).inMemoryJournalFrozen == []
+  requires I(jm).inMemoryJournal != []
+  ensures var (jm', s) := res;
+    && Inv(jm')
+    && JournalRangeOfByteSeq(s).Some?
+    && parseJournalRange(JournalRangeOfByteSeq(s).value) == Some(I(jm).inMemoryJournal)
+    && I(jm') == I(jm)
+          .(inMemoryJournal := [])
+          .(writtenLen := I(jm).writtenLen
+                + |JournalRangeOfByteSeq(s).value|)
+  {
+    var numBlocks := (jm.inMemoryWeight + 4064 - 1) / 4064;
+    var s := marshallJournalEntries(jm.journalEntries, jm.start, jm.len2, numBlocks);
+    var jm' := jm.(start := 0)
+                 .(len2 := 0)
+                 .(inMemoryWeight := 0)
+                 .(writtenJournalBlocks := jm.writtenJournalBlocks + numBlocks);
+    (jm', s)
+  }
+
+  function getWrittenJournalLen(jm: JournalistModel)
+      : (len : uint64)
+  requires Inv(jm)
+  ensures len as int == I(jm).writtenLen
+  {
+    jm.writtenJournalBlocks    
+  }
+
+  /*lemma roundUpOkay(a: int, b: int)
+  requires a <= 4064 * b
+  ensures ((a + 4064 - 1) / 4064) * 4064 <= 4064 * b
+  {
+  }*/
+
+  function {:opaque} freeze(jm: JournalistModel) : (jm' : JournalistModel)
+  requires Inv(jm)
+  requires I(jm).inMemoryJournalFrozen == []
+  requires I(jm).inMemoryJournal != []
+  ensures
+    && Inv(jm')
+    && I(jm') == I(jm)
+          .(inMemoryJournal := [])
+          .(inMemoryJournalFrozen :=
+              I(jm).inMemoryJournalFrozen + I(jm).inMemoryJournal)
+  {
+    jm.(len1 := jm.len1 + jm.len2)
+      .(len2 := 0)
+      .(frozenJournalBlocks := jm.frozenJournalBlocks + (jm.inMemoryWeight + 4064 - 1) / 4064)
+      .(inMemoryWeight := 0)
   }
 }
