ByteBlockCacheSystem/ByteSystem.i.dfy
@@ -1,0 +1,268 @@
+include "AsyncDiskModel.s.dfy"
+include "ByteCache.i.dfy"
+module ByteSystem refines AsyncDiskModel {
+  import M = ByteCache
+
+  import opened AsyncSectorDiskModelTypes
+  import opened Maps
+  import BC = BlockCache
+  import BJC = BlockJournalCache
+  import BJD = BlockJournalDisk
+  import opened DiskLayout
+  import opened JournalIntervals
+  import opened InterpretationDiskOps
+  import opened Options
+
+  function ReqReadWithLoc(reqReads: map<D.ReqId, D.ReqRead>, loc: Location) : Option<D.ReqId>
+  {
+    if id :| id in reqReads && LocOfReqRead(reqReads[id]) == loc then
+      Some(id)
+    else
+      None
+  }
+
+  function ReqWriteWithLoc(reqWrites: map<D.ReqId, D.ReqWrite>, loc: Location) : Option<D.ReqId>
+  {
+    if id :| id in reqWrites && LocOfReqWrite(reqWrites[id]) == loc then
+      Some(id)
+    else
+      None
+  }
+
+  function RespReadWithLoc(reqReads: map<D.ReqId, D.RespRead>, loc: Location) : Option<D.ReqId>
+  {
+    if id :| id in reqReads && LocOfRespRead(reqReads[id]) == loc then
+      Some(id)
+    else
+      None
+  }
+
+  function RespWriteWithLoc(reqWrites: map<D.ReqId, D.RespWrite>, loc: Location) : Option<D.ReqId>
+  {
+    if id :| id in reqWrites && LocOfRespWrite(reqWrites[id]) == loc then
+      Some(id)
+    else
+      None
+  }
+
+  //// Superblocks
+
+  predicate HasSuperblockAtLoc(disk: D.Variables, loc: Location)
+  {
+    && 0 <= loc.addr as int
+      <= loc.addr as int + loc.len as int
+      <= |disk.contents|
+    && ValidSuperblockBytes(
+        disk.contents[loc.addr .. loc.addr as int + loc.len as int])
+  }
+
+  function SuperblockAtLoc(disk: D.Variables, loc: Location) : Superblock
+  requires HasSuperblockAtLoc(disk, loc)
+  {
+    && SuperblockOfBytes(
+        disk.contents[loc.addr .. loc.addr as int + loc.len as int])
+  }
+
+  function SuperblockAtLocOpt(disk: D.Variables, loc: Location) : Option<Superblock>
+  {
+    if HasSuperblockAtLoc(disk, loc) then
+      Some(SuperblockAtLoc(disk,loc))
+    else
+      None
+  }
+
+  function ReqReadSuperblockAtLoc(disk: D.Variables, loc: Location) : Option<D.ReqId>
+  {
+    var id1 := ReqReadWithLoc(disk.reqReads, loc);
+    var id2 := RespReadWithLoc(disk.respReads, loc);
+    if id1.None? then id2 else id1
+  }
+
+  function ReqWriteSuperblockAtLoc(disk: D.Variables, loc: Location) : Option<JournalDisk.ReqWriteSuperblockId>
+  {
+    var id := ReqWriteWithLoc(disk.reqWrites, loc);
+    if id.Some? then
+      JournalDisk.ReqWriteSuperblockId(
+        id.value,
+        JournalDisk.ReqWriteSuperblock(SuperblockOfBytes(disk.reqWrites[id.value].bytes))
+      )
+    else (
+      var id2 := RespWriteWithLoc(disk.respWrites, loc);
+      if id2.Some? && HasSuperblockAtLoc(disk, loc) then
+        JournalDisk.ReqWriteSuperblockId(
+          id2.value,
+          JournalDisk.ReqWriteSuperblock(SuperblockAtLoc(disk, loc))
+        )
+      else
+        None
+    )
+  }
+
+  function Superblock1(disk: D.Variables) : Option<Superblock>
+  {
+    SuperblockAtLocOpt(disk, Superblock1Location())
+  }
+
+  function Superblock2(disk: D.Variables) : Option<Superblock>
+  {
+    SuperblockAtLocOpt(disk, Superblock2Location())
+  }
+
+  function ReqReadSuperblock1(disk: D.Variables) : Option<JournalDisk.ReqReadSuperblockId>
+  {
+    ReqReadSuperblock(disk, Superblock1Location())
+  }
+
+  function ReqReadSuperblock2(disk: D.Variables) : Option<JournalDisk.ReqReadSuperblockId>
+  {
+    ReqReadSuperblock(disk, Superblock2Location())
+  }
+
+  function ReqWriteSuperblock1(disk: D.Variables) : Option<JournalDisk.ReqWriteSuperblockId>
+  {
+    ReqWriteSuperblock(disk, Superblock1Location())
+  }
+
+  function ReqWriteSuperblock2(disk: D.Variables) : Option<JournalDisk.ReqWriteSuperblockId>
+  {
+    ReqWriteSuperblock(disk, Superblock2Location())
+  }
+
+  //// Journals
+
+  function ReqReadJournals_of_reqs(disk: D.Variables) : map<D.ReqId, JournalInterval>
+  {
+    map id | id in disk.reqReads &&
+        ValidJournalLocation(LocOfReqRead(disk.reqReads[id]))
+      :: JournalIntervalOfLocation(LocOfReqRead(disk.reqReads[id]))
+  }
+
+  function ReqReadJournals_of_resps(disk: D.Variables) : map<D.ReqId, JournalInterval>
+  {
+    map id | id in disk.respReads
+      && |disk.respReads[id].bytes| < 0x1_0000_0000_0000_0000
+      && ValidJournalLocation(LocOfRespRead(disk.respReads[id]))
+      :: JournalIntervalOfLocation(LocOfRespRead(disk.respReads[id]))
+  }
+
+  function ReqReadJournals(disk: D.Variables) : map<D.ReqId, JournalInterval>
+  {
+    MapUnion(
+        ReqReadJournals_of_reqs(disk), 
+        ReqReadJournals_of_resps(disk))
+  }
+
+  function ReqWriteJournals_of_reqs(disk: D.Variables) : map<D.ReqId, JournalInterval>
+  {
+    map id | id in disk.reqWrites
+      && |disk.reqWrites[id].bytes| < 0x1_0000_0000_0000_0000
+      && ValidJournalLocation(LocOfReqWrite(disk.reqWrites[id]))
+      :: JournalIntervalOfLocation(LocOfReqWrite(disk.reqWrites[id]))
+  }
+
+  function ReqWriteJournals_of_resps(disk: D.Variables) : map<D.ReqId, JournalInterval>
+  {
+    map id | id in disk.respWrites
+      && ValidJournalLocation(LocOfRespWrite(disk.respWrites[id]))
+      :: JournalIntervalOfLocation(LocOfRespWrite(disk.respWrites[id]))
+  }
+
+  function ReqWriteJournals(disk: D.Variables) : map<D.ReqId, JournalInterval>
+  {
+    MapUnion(
+        ReqWriteJournals_of_reqs(disk), 
+        ReqWriteJournals_of_resps(disk))
+  }
+
+  //// IndirectionTables
+
+  function ReqReadIndirectionTables_of_reqs(disk: D.Variables) : map<D.ReqId, Location>
+  {
+    map id | id in disk.reqReads &&
+        ValidIndirectionTableLocation(LocOfReqRead(disk.reqReads[id]))
+      :: LocOfReqRead(disk.reqReads[id])
+  }
+
+  function ReqReadIndirectionTables_of_resps(disk: D.Variables) : map<D.ReqId, Location>
+  {
+    map id | id in disk.respReads
+      && |disk.respReads[id].bytes| < 0x1_0000_0000_0000_0000
+      && ValidIndirectionTableLocation(LocOfRespRead(disk.respReads[id]))
+      :: LocOfRespRead(disk.respReads[id])
+  }
+
+  function ReqReadIndirectionTables(disk: D.Variables) : map<D.ReqId, Location>
+  {
+    MapUnion(
+        ReqReadIndirectionTables_of_reqs(disk), 
+        ReqReadIndirectionTables_of_resps(disk))
+  }
+
+  function ReqWriteIndirectionTables_of_reqs(disk: D.Variables) : map<D.ReqId, Location>
+  {
+    map id | id in disk.reqWrites
+      && |disk.reqWrites[id].bytes| < 0x1_0000_0000_0000_0000
+      && ValidIndirectionTableLocation(LocOfReqWrite(disk.reqWrites[id]))
+      :: LocOfReqWrite(disk.reqWrites[id])
+  }
+
+  function ReqWriteIndirectionTables_of_resps(disk: D.Variables) : map<D.ReqId, Location>
+  {
+    map id | id in disk.respWrites
+      && ValidIndirectionTableLocation(LocOfRespWrite(disk.respWrites[id]))
+      :: LocOfRespWrite(disk.respWrites[id])
+  }
+
+  function ReqWriteIndirectionTables(disk: D.Variables) : map<D.ReqId, Location>
+  {
+    MapUnion(
+        ReqWriteIndirectionTables_of_reqs(disk), 
+        ReqWriteIndirectionTables_of_resps(disk))
+  }
+
+  //// Nodes
+
+  function ReqReadNodes_of_reqs(disk: D.Variables) : map<D.ReqId, Location>
+  {
+    map id | id in disk.reqReads &&
+        ValidNodeLocation(LocOfReqRead(disk.reqReads[id]))
+      :: LocOfReqRead(disk.reqReads[id])
+  }
+
+  function ReqReadNodes_of_resps(disk: D.Variables) : map<D.ReqId, Location>
+  {
+    map id | id in disk.respReads
+      && |disk.respReads[id].bytes| < 0x1_0000_0000_0000_0000
+      && ValidNodeLocation(LocOfRespRead(disk.respReads[id]))
+      :: LocOfRespRead(disk.respReads[id])
+  }
+
+  function ReqReadNodes(disk: D.Variables) : map<D.ReqId, Location>
+  {
+    MapUnion(
+        ReqReadNodes_of_reqs(disk), 
+        ReqReadNodes_of_resps(disk))
+  }
+
+  function ReqWriteNodes_of_reqs(disk: D.Variables) : map<D.ReqId, Location>
+  {
+    map id | id in disk.reqWrites
+      && |disk.reqWrites[id].bytes| < 0x1_0000_0000_0000_0000
+      && ValidNodeLocation(LocOfReqWrite(disk.reqWrites[id]))
+      :: LocOfReqWrite(disk.reqWrites[id])
+  }
+
+  function ReqWriteNodes_of_resps(disk: D.Variables) : map<D.ReqId, Location>
+  {
+    map id | id in disk.respWrites
+      && ValidNodeLocation(LocOfRespWrite(disk.respWrites[id]))
+      :: LocOfRespWrite(disk.respWrites[id])
+  }
+
+  function ReqWriteNodes(disk: D.Variables) : map<D.ReqId, Location>
+  {
+    MapUnion(
+        ReqWriteNodes_of_reqs(disk), 
+        ReqWriteNodes_of_resps(disk))
+  }
+}
