Impl/JournalistMarshallingModel.i.dfy
@@ -1,0 +1,170 @@
+include "../ByteBlockCacheSystem/JournalBytes.i.dfy"
+include "../BlockCacheSystem/DiskLayout.i.dfy"
+
+module JournalistMarshallingModel {
+  import opened JournalRanges`Internal
+  import opened JournalBytes
+  import opened Journal
+  import opened DiskLayout
+  import opened NativeTypes
+  import opened Options
+  import opened Sequences
+  import opened Crypto
+
+  function {:opaque} cyclicSlice<T>(t: seq<T>, start: uint64, l: uint64) : (res: seq<T>)
+  requires 0 <= start as int < |t|
+  requires 0 <= l as int <= |t|
+  ensures l == 0 <==> res == []
+  {
+    if start as int + l as int <= |t| then
+      t[start .. start as int + l as int]
+    else
+      t[start ..] + t[.. start as int + l as int - |t| as int]
+  }
+
+  ///// Marshalling
+
+  lemma lemma_concatSeqJournalRangeLen(buf: seq<byte>, numBlocks: uint64)
+  requires |buf| == 4096 * numBlocks as int
+  ensures JournalRangeOfByteSeq(buf).Some?
+  ensures |concatSeq(JournalRangeOfByteSeq(buf).value)| == 4064 * numBlocks as int
+
+  function {:opaque} withoutChecksums(buf: seq<byte>, numBlocks: uint64) : (res: seq<byte>)
+  requires |buf| == 4096 * numBlocks as int
+  ensures  |res| == 4064 * numBlocks as int
+  {
+    lemma_concatSeqJournalRangeLen(buf, numBlocks);
+    concatSeq(JournalRangeOfByteSeq(buf).value)
+  }
+
+  function {:opaque} splice(bytes: seq<byte>, start: uint64, ins: seq<byte>) : (res: seq<byte>)
+  requires 0 <= start
+  requires start as int + |ins| <= |bytes|
+  requires |bytes| < 0x1_0000_0000_0000_0000
+  ensures |res| == |bytes|
+  {
+    bytes[.. start] + ins + bytes[start + |ins| as uint64 ..]
+  }
+
+  function {:opaque} writeOnto(buf: seq<byte>, numBlocks: uint64, start: uint64, bytes: seq<byte>)
+      : (buf' : seq<byte>)
+  requires |buf| == 4096 * numBlocks as int
+  requires numBlocks <= NumJournalBlocks()
+  requires |bytes| <= 4064
+  requires 0 <= start as int <= start as int + |bytes| <= 4064 * numBlocks as int
+  ensures |buf'| == |buf|
+  {
+    if |bytes| as uint64 > 0 then (
+      var block := start / 4064;
+      var idx := start % 4064;
+      assert start == block * 4064 + idx;
+      assert block < numBlocks;
+      if idx + |bytes| as uint64 <= 4064 then (
+        splice(buf, block * 4096 + 32 + idx, bytes)
+      ) else (
+        var buf1 := splice(buf, block * 4096 + 32 + idx, bytes[.. 4064 - idx]);
+        var buf2 := splice(buf1, (block + 1) * 4096 + 32, bytes[4064 - idx ..]);
+        buf2
+      )
+    ) else (
+      buf
+    )
+  }
+
+  lemma writeOntoResult(buf: seq<byte>, numBlocks: uint64, start: uint64, bytes: seq<byte>)
+  requires |buf| == 4096 * numBlocks as int
+  requires numBlocks <= NumJournalBlocks()
+  requires |bytes| <= 4064
+  requires 0 <= start as int <= start as int + |bytes| <= 4064 * numBlocks as int
+  ensures withoutChecksums(writeOnto(buf, numBlocks, start, bytes), numBlocks)
+        == splice(withoutChecksums(buf, numBlocks), start, bytes)
+
+  function writeIntOnto(buf: seq<byte>, numBlocks: uint64, idx: uint64, val: uint32) : (buf' : seq<byte>)
+  requires |buf| == 4096 * numBlocks as int
+  requires numBlocks <= NumJournalBlocks()
+  ensures |buf'| == |buf|
+
+  function writeHeader(buf: seq<byte>, numBlocks: uint64, len: uint64) : (buf' : seq<byte>)
+  requires |buf| == 4096 * numBlocks as int
+  requires 1 <= numBlocks <= NumJournalBlocks()
+  requires len <= 0xffff_ffff
+  ensures |buf'| == |buf|
+  {
+    var buf1 := writeIntOnto(buf, numBlocks, 0, len as uint32);
+    var buf2 := writeIntOnto(buf1, numBlocks, 4, numBlocks as uint32);
+    buf2
+  }
+
+  lemma lemma_cyclicRange_popFront_Sum(entries: seq<JournalEntry>, start: uint64, len: uint64)
+  requires |entries| < 0xfff_ffff_ffff_ffff
+  requires 0 <= start as int < |entries|
+  requires 1 <= len as int <= |entries|
+  ensures var start' := if start+1 == |entries| as uint64 then 0 else start+1;
+         SumJournalEntries(cyclicSlice(entries, start, len))
+      == SumJournalEntries(cyclicSlice(entries, start', len-1))
+            + WeightJournalEntry(entries[start]);
+
+  function {:opaque} writeJournalEntries(buf: seq<byte>, numBlocks: uint64, idx: uint64,
+      entries: seq<JournalEntry>, start: uint64, len: uint64) : (buf' : seq<byte>)
+  requires |buf| == 4096 * numBlocks as int
+  requires numBlocks <= NumJournalBlocks()
+  requires 0 <= start as int < |entries|
+  requires 0 <= len as int <= |entries|
+  requires |entries| < 0xfff_ffff_ffff_ffff
+  requires idx as int + SumJournalEntries(cyclicSlice(entries, start, len)) <= 4064 * numBlocks as int
+  ensures |buf'| == |buf|
+  decreases len
+  {
+    if len == 0 then
+      buf
+    else (
+      var start' := if start+1 == |entries| as uint64 then 0 else start+1;
+      lemma_cyclicRange_popFront_Sum(entries, start, len);
+
+      var buf0 := writeIntOnto(buf, numBlocks, idx, |entries[start].key| as uint32);
+      var idx0 := idx + 4;
+      var buf1 := writeOnto(buf0, numBlocks, idx0, entries[start].key);
+      var idx1 := idx0 + |entries[start].key| as uint64;
+      var buf2 := writeIntOnto(buf1, numBlocks, idx1, |entries[start].value| as uint32);
+      var idx2 := idx1 + 4;
+      var buf3 := writeOnto(buf2, numBlocks, idx2, entries[start].value);
+      var idx3 := idx2 + |entries[start].value| as uint64;
+      writeJournalEntries(buf3, numBlocks, idx3, entries, start', len - 1)
+    )
+  }
+
+  function {:opaque} fillInChecksums(buf: seq<byte>, numBlocks: uint64, i: uint64) : (buf' : seq<byte>)
+  requires |buf| == numBlocks as int * 4096
+  requires numBlocks <= NumJournalBlocks()
+  requires 0 <= i <= numBlocks
+  ensures |buf'| == |buf|
+  decreases numBlocks - i
+  {
+    if i == numBlocks then
+      buf
+    else (
+      var buf1 := splice(buf, 4096*i, Crc32C(buf[4096*i + 32 .. 4096*i + 4096]));
+      fillInChecksums(buf1, numBlocks, i+1)
+    )
+  }
+
+  function {:opaque} marshallJournalEntries(entries: seq<JournalEntry>,
+      start: uint64, len: uint64, numBlocks: uint64)
+    : (res: seq<byte>)
+  requires 0 <= start as int < |entries|
+  requires 0 <= len as int <= |entries|
+  requires |entries| <= 0xffff_ffff
+  requires WeightJournalEntries(cyclicSlice(entries, start, len)) <= 4064 * numBlocks as int
+  requires 1 <= numBlocks <= NumJournalBlocks()
+  ensures JournalRangeOfByteSeq(res).Some?
+  ensures parseJournalRange(JournalRangeOfByteSeq(res).value)
+       == Some(cyclicSlice(entries, start, len))
+  ensures |res| == numBlocks as int * 4096
+  {
+    var buf := fill((numBlocks * 4096) as int, 0);
+    var buf1 := writeHeader(buf, numBlocks, len);
+    var buf2 := writeJournalEntries(buf1, numBlocks, 8, entries, start, len);
+    var buf3 := fillInChecksums(buf2, numBlocks, 0);
+    buf3
+  }
+}
